Add partial proof of first result.
Several of the most major parts are missing, but the outline is now
present.

Moved the type inequality axioms to language, hint their use, and
improve them.

Add additional Axioms.v file encoding Coq-consistent global axioms.
Currently, this contains decidable type equality.

src/Result1.v
@@ -1,4 +1,4 @@
-From Pony Require Import Language Typing Heap Semantics.
+From Pony Require Import Axioms Language Typing Heap Semantics.
 
 Require Import Coq.FSets.FMapInterface.
 Require Import Coq.MSets.MSetInterface.
@@ -7,6 +7,24 @@ Require Import Coq.Structures.Equalities.
 Module Result1 (Map : WSfun) (SetM : WSetsOn).
 
 Module Sem := Semantics Map SetM.
+    
+
+Definition wellTypedLocals (gamma : Sem.WFExpr.context) (L : Sem.localVars) (chi : Sem.heap) : Prop :=
+  ( forall x : Syntax.var, 
+    forall S : Syntax.typeId,
+    forall b : Syntax.baseCapability,
+    forall v : Sem.value,
+      Sem.WFExpr.VarMapsTo x (Syntax.aType S b) gamma
+      -> Sem.LocalMap.VarMapsTo x v L
+      -> Sem.heapTyping v S chi)
+  /\ 
+  ( forall t : Syntax.temp,
+    forall S : Syntax.typeId,
+    forall k : Syntax.capability,
+    forall v : Sem.value,
+      Sem.WFExpr.TempMapsTo t (Syntax.type S k) gamma
+      -> Sem.LocalMap.TempMapsTo t v L
+      -> Sem.heapTyping v S chi).
 
 Theorem result1 :
   forall P : Sem.WFExpr.Program.program,
@@ -21,17 +39,86 @@ Theorem result1 :
   forall v : Sem.value,
     @Sem.WFExpr.typing P Syntax.expression gamma e (Syntax.type S k) gamma'
     -> @Sem.WFExpr.well_formed_expr P gamma (Syntax.seq e E) T
-    -> (forall x : Syntax.var, 
-        forall S' : Syntax.typeId,
-        forall b : Syntax.baseCapability,
-        forall v' : Sem.value,
-          Sem.WFExpr.VarMapsTo x (Syntax.aType S' b) gamma
-          -> Sem.LocalMap.VarMapsTo x v' L
-          -> Sem.heapTyping v' S' chi)
+    -> wellTypedLocals gamma L chi
     -> @Sem.evaluatesTo P Syntax.expression chi L e chi' L' v
     -> Sem.heapTyping v S chi'
         /\ @Sem.WFExpr.well_formed_expr P gamma' E T.
 Proof.
+  intros P gamma gamma' e E S k T L L' chi chi' v.
+
+  intros e_has_type_S_k e_seq_E_wf frame_well_typed e_evaluates_v.
+  
+  split.
+  (*Show that the evaluated value has the expected type.
+  *
+  * This depends on the form of the expression.
+  *)
+  { destruct e as [ newVar | var arhs | temp pf ].
+    { assert (v = None) as v_is_none.
+      { inversion e_evaluates_v.
+        contradict H; auto.
+        contradict H; auto.
+        contradict H; auto.
+        contradict H; auto.
+        contradict H; auto.
+        reflexivity.
+        { apply Coq.Logic.Eqdep_dec.inj_pair2_eq_dec in H4.
+          contradict H4.
+          discriminate.
+          apply Axioms.type_decidability.
+        }
+        contradict H; auto.
+        contradict H; auto. 
+      }
+      rewrite -> v_is_none.
+      apply Sem.heaptyp_null.
+    }
+    { admit. (* TODO *)
+    }
+    { admit. (* TODO *) 
+    }
+  }
+  (*Show the remaining expression is well-formed
+  *
+  * These are largely trivial, since a proof of the appropriate
+  * form is part of the inductive definition. The main work in each
+  * case requires arguing that the typing judgement is deterministic
+  * w.r.t. the output context, so that gamma' = gamma'0.
+  *)
+  { inversion e_seq_E_wf.
+    { assert (Syntax.type S k = t' /\ gamma' = gamma'0) as [ _ gamma_eq ].
+      { apply Sem.WFExpr.typing_func_on_type_and_outcome with (P:=P) (X:=Syntax.expression) (gamma:=gamma) (x:=Sem.WFExpr.varDecl x).
+        rewrite -> H.
+        assumption.
+        assumption.
+      }
+      rewrite -> gamma_eq; assumption.
+    }
+    { assert (Syntax.type S k = t' /\ gamma' = gamma'0) as [ _ gamma_eq ].
+      { apply Sem.WFExpr.typing_func_on_type_and_outcome with (P:=P) (X:=Syntax.expression) (gamma:=gamma) (x:=Sem.WFExpr.assign x arhs).
+        rewrite -> H.
+        assumption.
+        assumption.
+      }
+      rewrite -> gamma_eq; assumption.
+    }
+    { assert (Syntax.type S k = T' /\ gamma' = gamma'0) as [ _ gamma_eq ].
+      { apply Sem.WFExpr.typing_func_on_type_and_outcome with (P:=P) (X:=Syntax.expression) (gamma:=gamma) (x:=Sem.WFExpr.tempAssign t pf).
+        rewrite -> H.
+        assumption.
+        assumption.
+      }
+      rewrite -> gamma_eq; assumption.
+    }
+    { assert (Syntax.type S k = T' /\ gamma' = gamma'0) as [ _ gamma_eq ].
+      { apply Sem.WFExpr.typing_func_on_type_and_outcome with (P:=P) (X:=Syntax.expression) (gamma:=gamma) (x:=e).
+        assumption.
+        rewrite <- H.
+        assumption.
+      }
+      rewrite -> gamma_eq; assumption.
+    }
+  }
   Admitted.
 
 End Result1.
