src/Axioms.v
@@ -1,0 +1,5 @@
+Module Axioms.
+
+Axiom type_decidability : forall X Y : Type, { X = Y } + { X <> Y }.
+
+End Axioms.
